cleaned up TC and ex.

TypedCircuits.v
@@ -52,8 +52,7 @@ Inductive Pat : Ctx -> WType -> Set :=
          MergeCtx ctx1 ctx2 ctx
       -> Pat ctx1 w1
       -> Pat ctx2 w2
-      -> Pat ctx (Tensor w1 w2)
-.
+      -> Pat ctx (Tensor w1 w2).
 
 Inductive Unitary : WType -> Set := 
   | H : Unitary Qubit 
@@ -84,37 +83,54 @@ Inductive Circuit : Ctx -> WType -> Set :=
         -> Pat ctx1 w1
         -> (forall {ctx2 ctx2'}, MergeCtx ctx2 ctx ctx2' 
             -> Pat ctx2 w2 -> Circuit ctx2' w)
-        -> Circuit ctx1' w
-.
+        -> Circuit ctx1' w.
 
 Inductive Box : WType -> WType -> Set :=
 | box : forall {w1} {w2}, 
         (forall {ctx}, Pat ctx w1 -> Circuit ctx w2) -> Box w1 w2.
 
 Definition unbox {ctx} {w1} {w2} (b : Box w1 w2) : Pat ctx w1 -> Circuit ctx w2 :=
-  match b with
-    box f => f ctx
-  end.
+  match b with box f => f ctx end.
 
 End TC.
 Import TC.
 
 Open Scope type_scope.
 
-Definition Disjoint Γ1 Γ2 := {Γ : Ctx & MergeCtx Γ1 Γ2 Γ}.
-Definition Subset Γ1 Γ := {Γ2 : Ctx & MergeCtx Γ1 Γ2 Γ}.
+Definition disjoint Γ1 Γ2 := {Γ : Ctx & MergeCtx Γ1 Γ2 Γ}.
+Definition subset Γ1 Γ := {Γ2 : Ctx & MergeCtx Γ1 Γ2 Γ}.
 
-Lemma disjointEmptyL : forall Γ, Disjoint [] Γ.
+Infix "∥" := disjoint (at level 30).
+Infix "⊆" := subset (at level 30).
+
+Lemma disjoint_nil_l : forall Γ, [] ∥ Γ.
 Proof. intro. exists Γ. constructor. Qed.
 
-Lemma disjointEmptyR : forall Γ, Disjoint Γ [].
+Lemma disjoint_nil_r : forall Γ, Γ ∥ [].
 Proof. intro. exists Γ. constructor. Qed.
 
-Lemma disjointCons : forall o1 o2 o Γ1 Γ2,
-      MergeOption o1 o2 o -> Disjoint Γ1 Γ2 -> Disjoint (o1 :: Γ1) (o2 :: Γ2).
+Lemma disjoint_cons : forall o1 o2 o Γ1 Γ2,
+      MergeOption o1 o2 o -> Γ1 ∥ Γ2 -> (o1 :: Γ1) ∥ (o2 :: Γ2).
 Proof. destruct 2 as [Γ pfDisjoint]. exists (o :: Γ). constructor; auto. Qed.
 
-Lemma mergeOptionDisjoint : forall o1 o2 o3 o o',
+Lemma disjoint_cons_inv: forall (o1 o2 : option WType) (Γ1 Γ2 : Ctx),
+  (o1 :: Γ1) ∥ (o2 :: Γ2) -> Γ1 ∥ Γ2 * {o : (option WType) & MergeOption o1 o2 o}.
+Proof.
+  intros.
+  inversion H0.
+  inversion H1; subst.
+  split.
+  exists g. assumption.
+  exists o. assumption.
+Qed.
+
+Lemma merge_nil_l : forall Γ1 Γ2, MergeCtx [] Γ1 Γ2 -> Γ1 = Γ2.
+Proof. intros Γ1 Γ2 H. inversion H; subst; reflexivity. Qed.
+
+Lemma merge_nil_r : forall Γ1 Γ2, MergeCtx Γ1 [] Γ2 -> Γ1 = Γ2.
+Proof. intros Γ1 Γ2 H. inversion H; subst; reflexivity. Qed.
+
+Lemma merge_option_disjoint : forall o1 o2 o3 o o',
       MergeOption o1 o2 o -> MergeOption o o3 o' -> 
       {o0 : option WType  & MergeOption o1 o3 o0} 
     * {o0' : option WType & MergeOption o2 o3 o0'}.
@@ -124,31 +140,31 @@ Proof.
     try (exists (Some a); constructor).
 Qed.
 
-Lemma mergeDisjoint : forall Γ1 Γ2 Γ3 Γ Γ',
-      MergeCtx Γ1 Γ2 Γ -> MergeCtx Γ Γ3 Γ' -> Disjoint Γ1 Γ3 * Disjoint Γ2 Γ3.
+Lemma merge_disjoint : forall Γ1 Γ2 Γ3 Γ Γ',
+      MergeCtx Γ1 Γ2 Γ -> MergeCtx Γ Γ3 Γ' -> Γ1 ∥ Γ3 * Γ2 ∥ Γ3.
 Proof.
   intros ? ? ? ? ? merge_Γ1_Γ2_Γ merge_Γ_Γ3_Γ';
     revert Γ1 Γ2 merge_Γ1_Γ2_Γ.
   induction merge_Γ_Γ3_Γ' as [ | | o o3 o' Γ Γ3 Γ' merge_o_o3_o' merge_Γ_Γ3_Γ']; 
     intros Γ1 Γ2 merge_Γ1_Γ2_Γ;
     inversion merge_Γ1_Γ2_Γ; subst;
-    try (split; (apply disjointEmptyL || apply disjointEmptyR); fail).
-  - split; try apply disjointEmptyL.
+    try (split; (apply disjoint_nil_l || apply disjoint_nil_r); fail).
+  - split; try apply disjoint_nil_l.
     destruct (IHmerge_Γ_Γ3_Γ' Γ []) as [disjoint_g1_g2 _]; try constructor.
-    eapply disjointCons; eauto.
-  - split; try apply disjointEmptyL.
+    eapply disjoint_cons; eauto.
+  - split; try apply disjoint_nil_l.
     destruct (IHmerge_Γ_Γ3_Γ' Γ []) as [disjoint_g1_g2 _]; try constructor.
-    eapply disjointCons; eauto.
+    eapply disjoint_cons; eauto.
   - destruct (IHmerge_Γ_Γ3_Γ' _ _ H5).
-    edestruct (mergeOptionDisjoint o1 o2 o3) as [ [? ?] [? ?]]; eauto.
-    split; eapply disjointCons; eauto.
+    edestruct (merge_option_disjoint o1 o2 o3) as [ [? ?] [? ?]]; eauto.
+    split; eapply disjoint_cons; eauto.
 Qed.
 
-Lemma mergeOptionFunctional : forall o1 o2 o o',
+Lemma merge_option_functional : forall o1 o2 o o',
                               MergeOption o1 o2 o -> MergeOption o1 o2 o' -> o = o'.
 Proof. destruct 1; inversion 1; auto. Qed.
 
-Lemma mergeFunctional : forall {Γ1 Γ2 Γ Γ'}, 
+Lemma merge_functional : forall {Γ1 Γ2 Γ Γ'}, 
                  MergeCtx Γ1 Γ2 Γ -> MergeCtx Γ1 Γ2 Γ' -> Γ = Γ'.
 Proof.
   intros Γ1 Γ2 Γ Γ' merge_Γ1_Γ2_Γ.
@@ -157,23 +173,31 @@ Proof.
   - inversion merge_Γ1_Γ2_Γ'; auto.
   - inversion merge_Γ1_Γ2_Γ'; auto.
   - inversion merge_Γ1_Γ2_Γ'; subst.
-    erewrite mergeOptionFunctional with (o := o) (o' := o4); eauto.
+    erewrite merge_option_functional with (o := o) (o' := o4); eauto.
     rewrite IHmerge_Γ1_Γ2_Γ with (Γ' := g4); eauto.
 Qed.
 
-Lemma mergeOptionSymm : forall o1 o2 o, MergeOption o1 o2 o -> MergeOption o2 o1 o.
+Lemma merge_option_symm : forall o1 o2 o, MergeOption o1 o2 o -> MergeOption o2 o1 o.
 Proof. destruct 1; constructor. Qed.
 
-Lemma mergeSymm : forall {Γ1 Γ2 Γ}, MergeCtx Γ1 Γ2 Γ -> MergeCtx Γ2 Γ1 Γ.
-Proof. induction 1; constructor; auto. apply mergeOptionSymm; auto. Qed.
+Lemma merge_symm : forall {Γ1 Γ2 Γ}, MergeCtx Γ1 Γ2 Γ -> MergeCtx Γ2 Γ1 Γ.
+Proof. induction 1; constructor; auto. apply merge_option_symm; auto. Qed.
 
-Lemma mergeOptionAssoc : forall o1 o2 o3 o o' o0,
+Lemma disjoint_symm : forall Γ1 Γ2, Γ1 ∥ Γ2 -> Γ2 ∥ Γ1.
+Proof.
+  intros Γ1 Γ2 D.
+  destruct D as [Γ M].
+  apply merge_symm in M.  
+  exists Γ. assumption.
+Qed.
+
+Lemma merge_option_assoc : forall o1 o2 o3 o o' o0,
       MergeOption o1 o2 o -> MergeOption o o3 o'
    -> MergeOption o1 o3 o0
    -> MergeOption o2 o0 o'.
 Proof. inversion 1; inversion 1; inversion 1; constructor. Qed.
 
-Lemma mergeAssoc : forall Γ1 Γ2 Γ3 Γ Γ' Γ0,
+Lemma merge_assoc : forall Γ1 Γ2 Γ3 Γ Γ' Γ0,
       MergeCtx Γ1 Γ2 Γ -> MergeCtx Γ Γ3 Γ' 
    -> MergeCtx Γ1 Γ3 Γ0
    -> MergeCtx Γ2 Γ0 Γ'.
@@ -182,28 +206,28 @@ Proof.
   revert Γ3 Γ' Γ0.
   induction merge_Γ1_Γ2_Γ; intros Γ3 Γ' Γ0 merge_Γ_Γ3_Γ' merge_Γ1_Γ3_Γ0.
   - inversion merge_Γ1_Γ3_Γ0; subst; auto.
-  - rewrite (mergeFunctional merge_Γ_Γ3_Γ' merge_Γ1_Γ3_Γ0); constructor.
+  - rewrite (merge_functional merge_Γ_Γ3_Γ' merge_Γ1_Γ3_Γ0); constructor.
   - inversion merge_Γ1_Γ3_Γ0; subst; auto.
     * inversion merge_Γ_Γ3_Γ'; subst; auto.
-      constructor. apply mergeOptionSymm; auto. apply mergeSymm; auto.
+      constructor. apply merge_option_symm; auto. apply merge_symm; auto.
     * inversion merge_Γ_Γ3_Γ'; subst; auto.
       constructor.
-      + eapply mergeOptionAssoc; eauto.
+      + eapply merge_option_assoc; eauto.
       + eapply IHmerge_Γ1_Γ2_Γ; eauto.
 Qed.        
 
-Definition Merge3 Γ1 Γ2 Γ3 Γ := { Γ0 : Ctx & MergeCtx Γ1 Γ2 Γ0 * MergeCtx Γ0 Γ3 Γ}.
+Definition merge3 Γ1 Γ2 Γ3 Γ := { Γ0 : Ctx & MergeCtx Γ1 Γ2 Γ0 * MergeCtx Γ0 Γ3 Γ}.
 
-Lemma merge3Assoc : forall Γ1 Γ2 Γ3 Γ,
-                    Merge3 Γ1 Γ2 Γ3 Γ -> Merge3 Γ1 Γ3 Γ2 Γ.
+Lemma merge3_assoc : forall Γ1 Γ2 Γ3 Γ,
+                    merge3 Γ1 Γ2 Γ3 Γ -> merge3 Γ1 Γ3 Γ2 Γ.
 Proof.
   destruct 1 as [Γ0 [merge_Γ1_Γ2_Γ0 merge_Γ0_Γ3_Γ]].
-  assert (disjoint_Γ1_Γ3 : Disjoint Γ1 Γ3).
-    edestruct (mergeDisjoint Γ1 Γ2 Γ3); eauto.
+  assert (disjoint_Γ1_Γ3 : Γ1 ∥ Γ3).
+    edestruct (merge_disjoint Γ1 Γ2 Γ3); eauto.
   destruct disjoint_Γ1_Γ3 as [Γ0' merge_Γ1_Γ3_Γ0'].
   exists Γ0'. split; auto.
-  apply mergeSymm.
-  eapply (mergeAssoc Γ1 Γ2 Γ3); eauto.
+  apply merge_symm.
+  eapply (merge_assoc Γ1 Γ2 Γ3); eauto.
 Qed.
 
 Fixpoint compose {Γ1} {W} (c : Circuit Γ1 W)
@@ -221,24 +245,24 @@ Fixpoint compose {Γ1} {W} (c : Circuit Γ1 W)
   rename w into W1, w0 into W2, w1 into W;
   rename c0 into Γ01, c1 into Γ1, ctx into Γ0.
   rename pfM' into Merge_Γ01_Γ0_Γ1, pfM into Merge_Γ1_Γ_Γ1'.
-  edestruct (mergeDisjoint Γ01 Γ0 Γ) as [Disj_Γ01_Γ Disj_Γ0_Γ]; eauto.
+  edestruct (merge_disjoint Γ01 Γ0 Γ) as [Disj_Γ01_Γ Disj_Γ0_Γ]; eauto.
   destruct Disj_Γ0_Γ as [Γ0' Merge_Γ0_Γ_Γ0'].
   assert (Merge_Γ01_Γ0'_Γ1' : MergeCtx Γ01 Γ0' Γ1').
-    eapply mergeAssoc; eauto. apply mergeSymm; auto.
+    eapply merge_assoc; eauto. apply merge_symm; auto.
   refine (gate _ Merge_Γ01_Γ0'_Γ1' g p1 (fun Γ02 Γ02' Merge_Γ02_Γ0'_Γ02' q => _)).
-    edestruct (mergeDisjoint Γ0 Γ Γ02) as [[Γ002 Merge_Γ_Γ02_Γ002]
+    edestruct (merge_disjoint Γ0 Γ Γ02) as [[Γ002 Merge_Γ_Γ02_Γ002]
                                            [Γ02'' Merge_Γ0_Γ002_Γ02'']]; eauto;
-      try (eapply mergeSymm; eauto; fail).
+      try (eapply merge_symm; eauto; fail).
   refine (compose _ _ (h Γ02 Γ002 _ q) _ _ _ _ f);
-    try (apply mergeSymm; auto; fail).
+    try (apply merge_symm; auto; fail).
     (* Γ002 = Γ0 ⋓ Γ02 *)
     (* Γ02' = Γ02 ⋓ Γ0' = Γ02 ⋓ (Γ0 ⋓ Γ) *)
     (* So want to show that (Γ0 ⋓ Γ02) ⋓ Γ = Γ02 ⋓ (Γ0 ⋓ Γ) *)
-    assert (Merge3_Γ0_Γ_Γ02 : Merge3 Γ0 Γ Γ02 Γ02'). eexists.
-      constructor; eauto; try (apply mergeSymm; auto; fail).
-    apply merge3Assoc in Merge3_Γ0_Γ_Γ02.
+    assert (Merge3_Γ0_Γ_Γ02 : merge3 Γ0 Γ Γ02 Γ02'). eexists.
+      constructor; eauto; try (apply merge_symm; auto; fail).
+    apply merge3_assoc in Merge3_Γ0_Γ_Γ02.
     destruct Merge3_Γ0_Γ_Γ02 as [Γ002' [Merge_Γ0_Γ02_Γ002' Merge_Γ002'_Γ_Γ02']].
     assert (Γ002' = Γ002).
-      eapply mergeFunctional; eauto.
+      eapply merge_functional; eauto.
     subst. auto.
 Qed.
