Examples.v
@@ -7,22 +7,7 @@ Import TC.
 Import ListNotations.
 Open Scope list_scope.
 
-(* Untyped patterns *)
-Inductive UPat := uvar : Var -> UPat | uunit | upair : UPat -> UPat -> UPat.
-
-(* Untyped to typed *)
-Fixpoint make_singleton (v : Var) (W : WType) : Ctx := 
-  match v with
-  | O => [Some W]
-  | (S v') => None :: make_singleton v' W
-  end.
-
-Fixpoint make_SingletonCtx (v : Var) (W : WType) : 
-  SingletonCtx v W (make_singleton v W) :=
-  match v with
-  | O => SingletonHere W
-  | (S v') => SingletonLater _ _ _ (make_SingletonCtx v' W)
-  end.
+(** The merge function **)
 
 Fixpoint merge_atom (W1 W2 : option WType) : option WType := 
   match W1, W2 with
@@ -39,17 +24,9 @@ Fixpoint merge (ctx1 ctx2 : Ctx) : Ctx :=
     (merge_atom c1 c2) :: (merge ctx1' ctx2')
   end.
 
-Fixpoint make_context (p : UPat) (W : WType) : Ctx :=
-  match p with
-  | uvar v => make_singleton v W
-  | uunit => []
-  | upair p1 p2 => match W with 
-               | W1 ⊗ W2 => merge (make_context p1 W1) (make_context p2 W2)
-               | _ => [] (* Fails *)
-               end
-  end.
+Infix "∪" := merge (at level 30). 
 
-Lemma merge_eq : forall Γ1 Γ2 Γ3, MergeCtx Γ1 Γ2 Γ3 -> merge Γ1 Γ2 = Γ3.
+Lemma merge_eq : forall Γ1 Γ2 Γ3, MergeCtx Γ1 Γ2 Γ3 -> Γ1 ∪ Γ2 = Γ3.
 Proof.
   intros.
   generalize dependent Γ1. 
@@ -64,56 +41,122 @@ Proof.
     - simpl. 
       rewrite IHΓ3; trivial.
       inversion H5; reflexivity.
+Qed. 
+
+(* Have to rename to avoid conflicts *)
+Lemma merge_trans_l : forall Γ1 Γ2 Γ3 Γ4 Γ',
+  MergeCtx Γ1 Γ3 Γ' -> 
+  MergeCtx Γ2 Γ' Γ4 ->
+  MergeCtx (Γ1 ∪ Γ2) Γ3 Γ4.
+Proof.
+  intros Γ1 Γ2 Γ3 Γ4 Γ' H0 H1.
+  generalize dependent Γ'.
+  generalize dependent Γ4.
+  generalize dependent Γ3.
+  generalize dependent Γ1.
+  induction Γ2.
+  + intros Γ1 Γ3 Γ4 Γ' H0 H1. 
+    apply merge_nil_l in H1.
+    subst.
+    destruct Γ1; assumption.
+  + intros Γ1 Γ3 Γ4 Γ' H0 H1.
+    destruct Γ1.     
+    - simpl. 
+      apply merge_nil_l in H0; subst.
+      assumption.
+    - simpl. 
+      inversion H0; subst.
+      * inversion H1; subst.
+        apply merge_symm in H1.
+        apply merge_eq in H1.
+        simpl in H1. rewrite H1.
+        constructor.
+      * inversion H1; subst.
+        destruct o, a, o2, o4; inversion H4; subst; inversion H9; subst; simpl in *;
+        constructor; try constructor; eapply IHΓ2; try apply H7; try apply H10.
 Qed.
 
-(* Can turn into a function that returns an Option?
-Program Fixpoint type_pat (p : UPat) (W : WType) : (Pat (make_context p W) W) :=
-  match p with
-  | uvar v => var _ _ _ (make_SingletonCtx v W)
-  | uunit => unit 
-  | upair p1 p2 => match W with 
-                  | W1 ⊗ W2 => pair _ _ _ _ _ _ (type_pat p1 W1) (type_pat p2 W2)
-                  | _ => unit (* Really Fails *)
-                  end
-  end. 
-Next Obligation. 
-*)
+Lemma merge_trans_r : forall Γ1 Γ2 Γ3 Γ4 Γ',
+  MergeCtx Γ1 Γ2 Γ' -> 
+  MergeCtx Γ3 Γ' Γ4 ->
+  MergeCtx Γ1 (Γ2 ∪ Γ3) Γ4.
+Proof.
+  intros Γ1 Γ2 Γ3 Γ4 Γ' H0 H1.
+  apply merge_symm.
+  eapply merge_trans_l.
+  apply (merge_symm H0).
+  apply H1.
+Qed.  
 
-(* Alternatives for simple patterns *)
+Lemma manual_merge_symm : forall Γ1 Γ2, Γ1 ∪ Γ2 = Γ2 ∪ Γ1.
+Proof.
+  intros Γ1. 
+  induction Γ1; intros Γ2.
+  destruct Γ2; reflexivity.  
+  destruct Γ2; trivial.
+  simpl. 
+  rewrite IHΓ1.
+  destruct a, o; reflexivity.
+Qed.
 
-(*
-Definition type_var (v : Var) (W : WType) : Pat (make_singleton v W) W :=
-  var _ _ _ (make_SingletonCtx v W).
+Lemma manual_merge_assoc : forall Γ1 Γ2 Γ3, 
+  Γ1 ∥ Γ2 ->
+  Γ2 ∥ Γ3 ->
+  (Γ1 ∪ Γ2) ∪ Γ3 = Γ1 ∪ (Γ2 ∪ Γ3).
+Proof.
+  intros Γ1 Γ2.
+  generalize dependent Γ1.
+  induction Γ2.
+  + intros; simpl.
+    destruct Γ1; reflexivity.
+  + intros; simpl.
+    destruct Γ1, Γ3; simpl; trivial.
+    rewrite IHΓ2.
+    - destruct o, a, o0; trivial.
+      inversion H0.
+      inversion H2; subst.
+      inversion H8.    
+    - inversion H0.
+      inversion H2; subst.
+      exists g. assumption.
+    - inversion H1.
+      inversion H2; subst.
+      exists g. assumption.
+Qed.
 
+Lemma disjoint_merge : forall Γ1 Γ2, Γ1 ∥ Γ2 -> MergeCtx Γ1 Γ2 (Γ1 ∪ Γ2).
+Proof.
+  intros Γ1 Γ2 H0.
+  unfold disjoint in H0.
+  destruct H0.
+  specialize (merge_eq _ _ _ m); intros; subst.
+  assumption.
+Qed.
 
-Search (_ <> _) bool.
-
-Program Definition type_pair (v1 v2 : Var) (W1 W2 : WType) {pf : (v1 =? v2) = false}: 
-  Pat (make_context (upair (uvar v1) (uvar v2)) (W1 ⊗ W2)) (W1 ⊗ W2) :=
-  pair _ _ _ _ _ _ (type_var v1 W1) (type_var v2 W2).
-Obligation 1. 
-  apply Nat.eqb_neq in pf. 
-  generalize dependent v2.
-  induction v1; intros.
-  destruct v2. tauto.
-  simpl; apply MergeCons; constructor.
-  simpl.
-  destruct v2.
-  simpl. apply MergeCons. constructor.
-  destruct (make_singleton v1 W1); simpl; constructor.
-  simpl.
-  constructor.
-  constructor.
-  apply IHv1.
-  intros Eq; subst; tauto.
-Defined.
-*)
-
+Lemma pairwise_disjoint : forall Γ1 Γ2 Γ3, 
+  Γ1 ∥ Γ2 -> Γ2 ∥ Γ3 -> Γ1 ∥ Γ3 -> (Γ1 ∪ Γ2) ∥ Γ3.
+Proof.
+  intros Γ1 Γ2. generalize dependent Γ1.
+  induction Γ2; intros.
+  + destruct Γ1; simpl; assumption. 
+  + destruct Γ1, Γ3; simpl; trivial.
+    - apply disjoint_nil_r.
+    - apply disjoint_cons_inv in H0 as [D12 [o12 mo12]].
+      apply disjoint_cons_inv in H1 as [D23 [o23 mo23]].
+      apply disjoint_cons_inv in H2 as [D13 [o13 mo13]].
+      apply disjoint_cons with (o := merge_atom o12 o0) .
+      destruct o, a, o0; inversion mo12; inversion mo23; inversion mo13; subst;
+      simpl; constructor.
+      apply IHΓ2; assumption.
+Qed.      
+        
 (* Projecting out elements of tensors *)
 Program Definition wproj {Γ W1 W2} (p : Pat Γ (Tensor W1 W2)) : 
   {Γ1 : Ctx & Pat Γ1 W1 } * {Γ2 : Ctx & Pat Γ2 W2} :=
   match p with 
   | unit => _
+  | qubit _ _ _ => _
+  | bit _ _ _ => _
   | pair ctx1 ctx2 ctx w1 w2 M' p1 p2 => (existT _ ctx1 p1, existT _ ctx2 p2)  
   end.
 
@@ -131,141 +174,53 @@ Qed.
 
 (* Dangerous to take this notation *)
 Notation "a , b" := (Datatypes.pair a b) (at level 11, left associativity) : default_scope.
-(*
-Notation "w1 , w2" := (upair w1 w2) (at level 11, left associativity) : circ_scope.
-*)
-
 Notation "w1 , w2" := (pair _ _ _ _ _ _ w1 w2) (at level 11, left associativity) : circ_scope.
-
 Notation "(())" := unit : circ_scope.
 
+Parameter Δ1 Δ2 Δ3 Δ4 Δ5 Δ6 Δ7: Ctx.
 
-(* Some wire patterns *)
-Definition q : Var := 0.
-Definition w : Var  := 1.
-Definition w': Var  := 2.
-Definition a : Var  := 3.
-Definition b : Var  := 4.
-Definition x : Var  := 5.
-Definition y : Var  := 6.
-Definition w1 : Var := 7.
-Definition w1': Var := 8.
-Definition w2 : Var := 9.
-Definition w2': Var := 10.
-
-Check q.
-Check w1.
- 
 (* Getting contexts for input patterns *)
 
 Open Scope circ_scope.
 
 (*** Tactics ***)
 
-Lemma merge_l_eq : forall Γ1 Γ2, MergeCtx [] Γ1 Γ2 -> Γ1 = Γ2.
-Proof. intros Γ1 Γ2 H. inversion H; subst; reflexivity. Qed.
-
-Lemma merge_r_eq : forall Γ1 Γ2, MergeCtx Γ1 [] Γ2 -> Γ1 = Γ2.
-Proof. intros Γ1 Γ2 H. inversion H; subst; reflexivity. Qed.
-
-Ltac find_pat := 
-  repeat match goal with 
-  | [ H : ?P |- ?P ] => exact H
-  | [ H : MergeCtx [] ?Γ1 ?Γ2 |- _] => apply merge_l_eq in H; subst
-  | [ H : MergeCtx ?Γ1 [] ?Γ2 |- _] => apply merge_r_eq in H; subst
-  end.
+(* Prevent compute from unfolding important fixpoints *)
+Opaque merge.
+Opaque wproj.
+Opaque Ctx.
 
 Ltac type_check_circ := 
   intros;
-  compute;
-  (* Compute in hyps will screw things up here *)
-  repeat match goal with 
-  | [ H : _  = wproj ?p |- _ ]      => apply wproj_merge in H
-  end;
   compute in *;
   repeat match goal with 
+  | [ |- Ctx ]                      => simpl (* do not try random ctx or permute goal *)
   | [ |- ?Γ = ?Γ ]                  => reflexivity
-  (* from find_pat *)
-  | [ H : ?P |- ?P ]                => exact H
-  | [ H : MergeCtx [] ?Γ1 ?Γ2 |- _] => apply merge_l_eq in H; subst 
-  | [ H : MergeCtx ?Γ1 [] ?Γ2 |- _] => apply merge_r_eq in H; subst
-  | [ H : MergeCtx ?Γ1 ?Γ2 ?Γ3 |- MergeCtx ?Γ2 ?Γ1 ?Γ3 ] => apply (mergeSymm H)
+  | [ H : MergeCtx ?Γ1 ?Γ2 ?Γ3 |- MergeCtx ?Γ1 ?Γ2 ?Γ3 ] => exact H
+  | [ H : MergeCtx ?Γ1 ?Γ2 ?Γ3 |- MergeCtx ?Γ2 ?Γ1 ?Γ3 ] => apply (merge_symm H)
+  | [ H : _  = wproj ?p |- _ ]      => apply wproj_merge in H
+  | [ H : MergeCtx [] ?Γ1 ?Γ2 |- _] => apply merge_nil_l in H; subst 
+  | [ H : MergeCtx ?Γ1 [] ?Γ2 |- _] => apply merge_nil_r in H; subst
+  | [ p : Pat ?Γ One |- _ ]         => inversion p; subst; clear p
   | [ |- Pat [] One ]               => apply unit
   | [ |- SingletonCtx _ ?W (?C :: [])]  => apply SingletonHere
   | [ |- SingletonCtx _ ?W (None :: _)] => apply SingletonLater
-  (* From context checking *)
   | [ |- MergeCtx [] _ _]           => apply MergeNilL
   | [ |- MergeCtx _ [] _]           => apply MergeNilR
   | [ |- MergeCtx _ _ []]           => apply MergeNilL (* Both work *)
   end.
 
-(* Should be element of, but company coq is annoying *)
-(* Infix " ⊂ " := get_context (at level 50). *)
-
-(*
-Notation "'Box' w ⊂ W => C" := (box (make_context w W) w C _ _) (at level 60) 
-                               : circ_scope.
-*)
-
-(*
-Definition out (v : Var) (W : WType ) := output (type_var v W).
-*)
 
 (*** Paper Examples ***)
 
-(* Local Obligation Tactic := type_check_circ. *)
-
-(* I don't like having to specify these at all. 
-   It basically means no more variables. *)
-
-(* Program Definition id_circ : Circuit [Some Qubit] Qubit := output _.
-Next Obligation. type_check_circ. Defined. *)
+Local Obligation Tactic := type_check_circ.
 
 Program Definition id_circ {W} :  Box W W := 
   box (fun Γ p1 => output p1).
 
-
 (*
 Program Definition id_circ' : Circuit _ _ := 
   output (type_var q Qubit).
-*)
-
-(*
-Program Definition id_circ : Circuit _ _ := out w Qubit. 
-*)
-
-Check id_circ.
-Print id_circ.
-Eval simpl in id_circ.
-Eval compute in id_circ.
-
-(*
-Eval compute in id_circ'.
-*)
-
-(*
-Program Definition hadamard_c : Circuit [Some Qubit] Qubit :=
-  gate [] H (type_var q Qubit) (fun Γ2 Γ2' M2 p2 => output p2) _ .
-Next Obligation. type_check_circ. Defined.
-Next Obligation. type_check_circ. Defined.
-(*
-Next Obligation. apply merge_r_eq in H1. subst. assumption. Defined.
-Next Obligation. apply MergeNilR. Defined.
-*)
-
-(* Doesn't work. Why not?
-Program Definition hadamard_c : Circuit [Some Qubit] Qubit :=
-  gate [] H (make_pattern q Qubit) (fun _ _ _ _ => output (make_pattern q Qubit)) _ .
-Next Obligation. type_check_circ. Defined.
-Next Obligation. type_check_circ. Defined. *)
-
-Program Definition hadamard_measure_c : Circuit [Some Qubit] Bit :=
-  gate [] H (type_var q Qubit) 
-  (fun Γ2 Γ2' M2 p2 => gate [] meas p2
-  (fun Γ3 Γ3' M3 p3 => output p3) _) _ .
-Next Obligation. type_check_circ. Defined.
-
-Check box.
 *)
 
 Program Definition hadamard_measure : Box Qubit Bit :=
@@ -273,49 +228,23 @@ Program Definition hadamard_measure : Box Qubit Bit :=
    gate [] _ H p1 
   (fun Γ2 Γ2' M2 p2 => gate [] _ meas p2
   (fun Γ3 Γ3' M3 p3 => output p3))).
-Next Obligation. type_check_circ. Defined.
-Next Obligation. type_check_circ. Defined.
-  
-(* This - correctly - fails to type check!*)
-(*
-Program Definition absurd_circ : Boxed_Circ Qubit (Bit ⊗ Qubit) := 
-  Box w ⊂ Qubit =>
-    (gate meas w x 
-    (gate H w w'
-    (output (x,w')))).
-Obligation 2. Abort. 
-*)
 
-(*
-Program Definition inSeq {W1 W2 W3 : WType} 
-  (c1 : Boxed_Circ W1 W2) (c2 : Boxed_Circ W2 W3) : Boxed_Circ W1 W3  := 
-  Box w1 ⊂ W1 =>
-    (compose w2 (unbox c1 w1) (unbox c2 w2)).
-Obligation 2. type_check_circ. Admitted. (* subst not yet defined *)
+Program Definition inSeq {W1 W2 W3} (c1 : Box W1 W2) (c2 : Box W2 W3) : Box W1 W3  := 
+  box (fun Γ1 p1 => @compose Γ1 W2 (unbox c1 p1) [] Γ1 W3 _ 
+                                (fun Γ2 Γ2' M2 p2 => unbox c2 p2)). 
 
-Program Definition inPar {W1 W2 W1' W2'} 
-  (c : Boxed_Circ W1 W2) (c' : Boxed_Circ W1' W2') : Boxed_Circ (W1⊗W1') (W2⊗W2') :=
-  Box (w1,w1') ⊂ (W1 ⊗ W1') =>
-    (compose w2 (unbox c w1) (
-       compose w2 (unbox c' w1') (output (w2,w2')))).
-Obligation 2. type_check_circ. Admitted. (* subst not yet defined *)
-*)
+Program Definition inPar {W1 W2 W1' W2'} (c1 : Box W1 W1') (c2 : Box W2 W2') : 
+  Box (W1⊗W2) (W1'⊗W2') :=
+  box (fun Γ12 p12 => 
+   match wproj p12 with Datatypes.pair (existT _ Γ1 p1) (existT _ Γ2 p2) =>
+   @compose Γ1 W1' (unbox c1 p1) Γ2 Γ12 (W1'⊗W2') _
+                   (fun Γ3 Γ3' M3 p1' => @compose Γ2 W2' (unbox c2 p2) Γ3 Γ3' (W1'⊗W2')
+                                       _ (fun Γ4 Γ4' M4 p2' => (output (p1',p2')))) 
+   end).
 
-Program Definition init : Box One Qubit :=
+Program Definition init (b : bool) : Box One Qubit :=
   if b then (box (fun Γ p1 => gate [] _ init1 p1 (fun Γ2 Γ2' M2 p2 => output p2)))
        else (box (fun Γ p1 => gate [] _ init0 p1 (fun Γ2 Γ2' M2 p2 => output p2))).
-Next Obligation. type_check_circ. Defined.
-Next Obligation. type_check_circ. Defined.
-Next Obligation. type_check_circ. Defined.
-Next Obligation. type_check_circ. Defined.
-
-(*
-Program Definition init (b : bool) : Boxed_Circ One Qubit := 
-  if b then (Box unit ⊂ One => (gate init1 unit w (output w)))
-       else (Box unit ⊂ One => (gate init0 unit w (output w))).
-*)
-
-Parameter Δ1 Δ2 Δ3 Δ4 Δ5 : Ctx.
 
 Program Definition bell00 : Box One (Qubit ⊗ Qubit) :=
 (* I don't like this. Would be much simpler if I could force Γ = [] *)
@@ -325,36 +254,7 @@ Program Definition bell00 : Box One (Qubit ⊗ Qubit) :=
   (fun Γ3 Γ3' M3 p3 => gate Γ3 _ (* Γ2'? *) H p2
   (fun Γ4 Γ4' M4 p4 => gate [] _ CNOT (p3,p4) 
   (fun Γ5 Γ5' M5 p5 => output p5)))))).
-Next Obligation. type_check_circ. Defined.
-Next Obligation. type_check_circ. Defined.
-Next Obligation. type_check_circ. Defined.
-Next Obligation. type_check_circ. Defined.
-Next Obligation. type_check_circ. Defined.
-Next Obligation. type_check_circ. Defined.
-
-(*
-Program Definition bell00' : Box One (Qubit ⊗ Qubit) :=
-(* I don't like this. Would be much simpler if I could force Γ = [] *)
-  box (fun Γ p1 => 
-  (gate Γ init0 (())
-  (fun Γ2 Γ2' M2 p2 => gate (merge Γ2 Γ) init0 (())
-  (fun Γ3 Γ3' M3 p3 => gate (merge Γ3 Γ) (* Γ2'? *) H p2
-  (fun Γ4 Γ4' M4 p4 => gate Δ4 CNOT (p3,p4) 
-  (fun Γ5 Γ5' M5 p5 => output p5) _ ) _) _) _)).
-Obligation 7. type_check_circ. Defined.
-Obligation 6. erewrite merge_eq. constructor. assumption. Defined.
-Obligation 5. type_check_circ.
-*)  
-
-(*
-Program Definition bell00 : Boxed_Circ One (Qubit ⊗ Qubit) :=
-  Box unit ⊂ One =>
-    (gate init0 unit a
-    (gate init0 unit b
-    (gate H a a
-    (gate CNot (a,b) (a,b)
-    (output (a,b)))))).
-*)
+Next Obligation. apply Γ4'. Defined.
 
 (* Work in progress *)
 Notation "⟨ p1 , p2 , Γ1 , Γ2 ⟩ ↩ p $ exp" := match wproj p with 
@@ -364,170 +264,73 @@ Program Definition alice : Box (Qubit⊗Qubit) (Bit⊗Bit) :=
   box (fun Γ qa => 
   (gate [] _ CNOT qa
   (fun Γ2 Γ2' M2 p2 => match wproj p2 with Datatypes.pair (existT _ Γq q) (existT _ Γa a) =>
-  (*  let ((existT _ Γ1'' q), (existT _ Γ2'' a)) := wproj p2 in *)
      gate Γa _ H q
   (fun Γ3 Γ3' M3 p3 => gate Γa _ meas p3
   (fun Γ4 Γ4' M4 p4 => gate Γ4 _ meas a 
   (fun Γ5 Γ5' M5 p5 => output (p4,p5)))) 
 end))).
-Next Obligation. type_check_circ. Defined.
-Next Obligation. type_check_circ. Defined.
-Next Obligation. type_check_circ. Defined.
-Next Obligation. type_check_circ. Defined.
-
-(*
-Program Definition alice : Boxed_Circ (Qubit⊗Qubit) (Bit⊗Bit) :=
-  Box (q,a) ⊂ Qubit⊗Qubit =>
-    (gate CNot (q,a) (q,a)
-    (gate H q q
-    (gate meas q x
-    (gate meas a y
-    (output (x,y)))))).
-*)
-
-(* Have to rename to avoid conflicts *)
-Lemma merge_trans_l : forall Γ1 Γ2 Γ3 Γ4 Γ',
-  MergeCtx Γ1 Γ3 Γ' -> 
-  MergeCtx Γ2 Γ' Γ4 ->
-  MergeCtx (merge Γ1 Γ2) Γ3 Γ4.
-Proof.
-  intros Γ1 Γ2 Γ3 Γ4 Γ' H0 H1.
-  generalize dependent Γ'.
-  generalize dependent Γ4.
-  generalize dependent Γ3.
-  generalize dependent Γ1.
-  induction Γ2.
-  + intros Γ1 Γ3 Γ4 Γ' H0 H1. 
-    apply merge_l_eq in H1.
-    subst.
-    destruct Γ1; assumption.
-  + intros Γ1 Γ3 Γ4 Γ' H0 H1.
-    destruct Γ1.     
-    - simpl. 
-      apply merge_l_eq in H0; subst.
-      assumption.
-    - simpl. 
-      inversion H0; subst.
-      * inversion H1; subst.
-        apply mergeSymm in H1.
-        apply merge_eq in H1.
-        simpl in H1. rewrite H1.
-        constructor.
-      * inversion H1; subst.
-        destruct o, a0, o2, o4; inversion H4; subst; inversion H9; subst; simpl in *;
-        constructor; try constructor; eapply IHΓ2; try apply H7; try apply H10.
-Qed.
-
-Lemma merge_trans_r : forall Γ1 Γ2 Γ3 Γ4 Γ',
-  MergeCtx Γ1 Γ2 Γ' -> 
-  MergeCtx Γ3 Γ' Γ4 ->
-  MergeCtx Γ1 (merge Γ2 Γ3) Γ4.
-Proof.
-  intros Γ1 Γ2 Γ3 Γ4 Γ' H0 H1.
-  apply mergeSymm.
-  eapply merge_trans_l.
-  apply (mergeSymm H0).
-  apply H1.
-Qed.  
-
-Lemma manual_merge_symm : forall Γ1 Γ2, merge Γ1 Γ2 = merge Γ2 Γ1.
-Proof.
-  intros Γ1. 
-  induction Γ1; intros Γ2.
-  destruct Γ2; reflexivity.  
-  destruct Γ2; trivial.
-  simpl. 
-  rewrite IHΓ1.
-  destruct a0, o; reflexivity.
-Qed.
 
 Program Definition bob : Box (Bit⊗Bit⊗Qubit) Qubit :=
   box (fun Γxyb xyb =>
-    match wproj xyb with Datatypes.pair (existT _ Γx x) (existT _ Γyb yb) =>
-    gate Δ1 _ (bit_control σx) yb 
+    match wproj xyb with Datatypes.pair (existT _ Γxy xy) (existT _ Γb b) =>
+    match wproj xy with Datatypes.pair (existT _ Γx x) (existT _ Γy y) =>
+    gate Γx _ (bit_control σx) (y,b) 
      (fun Γyb Γyb' Myb yb =>
-      match wproj yb with Datatypes.pair (existT _ Γy y) (existT _ Γb b) =>
-      gate Δ2 _ (bit_control σz) (x,b)
+      match wproj yb with Datatypes.pair (existT _ Γy' y') (existT _ Γb' b') =>
+      gate Γy' _ (bit_control σz) (x,b')
        (fun Γxb Γxb' Mxb xb =>
-        match wproj xb with Datatypes.pair (existT _ Γx x) (existT _ Γb b) =>
-        gate Δ3 _ discard y 
+        gate Γxb _ discard y' 
          (fun Γz1 Γz1 Mz1 z1 =>
-          gate Δ4 _ discard x
-          (fun Γz2 Γz2' Mz2 z2 => output b))
-        end)
+          match wproj xb with Datatypes.pair (existT _ Γx' x') (existT _ Γb'' b'') =>
+          gate Γb'' _ discard x'
+           (fun Γz2 Γz2' Mz2 z2 => output b'')
+          end))
       end)
+    end
     end).
+Next Obligation. apply (merge Γy Γb). Defined.
+Next Obligation. eapply merge_trans_l.
+                 apply (merge_symm Heq_anonymous). 
+                 apply (merge_symm Heq_anonymous0). Defined.
+Next Obligation. specialize (merge_disjoint _ _ _ _ _ Heq_anonymous Heq_anonymous0). 
+                 intros [D1 D2].
+                 apply disjoint_merge.
+                 assumption. Defined.
+Next Obligation. apply (merge Γb' Γx). Defined.
+Next Obligation. eapply merge_trans_l.
+                 apply (merge_symm Heq_anonymous). 
+                 apply (merge_symm Myb). Defined.
+Next Obligation. apply merge_symm.
+                 specialize (merge_disjoint _ _ _ _ _ Heq_anonymous Myb). 
+                 intros [D1 D2].
+                 apply disjoint_merge.
+                 assumption. Defined.
 
-
-
-
-Program Definition bob : Box (Bit⊗Bit⊗Qubit) Qubit :=
-  box (fun Γxyb xyb =>
-    match wproj xyb with Datatypes.pair (existT _ Γx x) (existT _ Γyb yb) =>
-    gate Γx _ (bit_control σx) yb 
-     (fun Γyb Γyb' Myb yb =>
-      match wproj yb with Datatypes.pair (existT _ Γy y) (existT _ Γb b) =>
-      gate (merge Γx Γy) _ (bit_control σz) (x,b)
-       (fun Γ2 Γ2' M2 p2 =>
-        match wproj p2 with Datatypes.pair (existT _ Γx x) (existT _ Γb b) =>
-        gate Δ3 _ discard y 
-         (fun Γ3 Γ3' M3 p3 =>
-          gate Δ4 _ discard x
-          (fun Γ4 Γ4' M4 p4 => output b))
-        end)
-      end)
-    end).
-Next Obligation. type_check_circ. Defined.
-Next Obligation. unfold bob_obligation_2. 
-                 apply wproj_merge in Heq_anonymous.
-                 apply wproj_merge in Heq_anonymous0.
-                 clear - Heq_anonymous Heq_anonymous0 Myb.
-                 rewrite manual_merge_symm.
-                 eapply merge_trans_r.
-                 apply (mergeSymm Heq_anonymous).
-                 apply (mergeSymm Myb). Defined.                 
-Next Obligation. type_check_circ.
-                 clear - Heq_anonymous Heq_anonymous0 Myb.
-                 
-
-
-
-Program Definition bob : Boxed_Circ (Bit⊗Bit⊗Qubit) Qubit :=
-  Box (x,y,b) ⊂ (Bit⊗Bit⊗Qubit) =>
-    (gate (bit_control σx) (y,b) (y,b)
-    (gate (bit_control σz) (x,b) (x,b)
-    (gate discard y unit 
-    (gate discard x unit
-    (output b))))).
-
-Program Definition teleport : Boxed_Circ Qubit Qubit :=
-  Box q ⊂ Qubit =>
-    (compose (a,b) (unbox bell00 unit)
-    (compose (x,y) (unbox alice (q,a))
-    (unbox bob (x,y,b)))).
-Obligation 2. type_check_circ. Admitted.
-
-(* For when run is implemented: *)
-
-Parameter run : Circuit -> bool.
-
-Parameter run2 : Boxed_Circ One Bit -> bool.
-
-Program Definition flip : bool := 
-  run 
-  (gate init0 unit q
-  (gate H q q
-  (gate meas q b
-  (output b)))).
-
-
-Program Definition flip2 : bool := 
-  run2 
-  (Box unit ⊂ One => 
-  (gate init0 unit q
-  (gate H q q
-  (gate meas q b
-  (output b))))).
-
+Program Definition teleport : Box Qubit Qubit :=
+  box (fun Γq q =>
+    @compose [] (Qubit⊗Qubit) (unbox bell00 unit) Γq Γq Qubit _
+      (fun Γab Γab' Mab ab => 
+       match wproj ab with Datatypes.pair (existT _ Γa a) (existT _ Γb b) =>
+       @compose (merge Γq Γa) (Bit⊗Bit) (unbox alice (q,a)) Γb (merge Γq Γab) Qubit _
+         (fun Γxy Γxy' Mxy xy => unbox bob (xy,b))
+       end)
+      ).
+Next Obligation. apply disjoint_merge.
+                 apply disjoint_symm.
+                 eapply merge_disjoint.
+                 apply (merge_symm Heq_anonymous).
+                 apply Mab. Defined.
+Next Obligation. assert (Γa ∥ Γb) as Dab.
+                   exists Γab. assumption.
+                 specialize (merge_disjoint _ _ _ _ _ Heq_anonymous Mab).
+                 intros [Daq Dbq].
+                 apply merge_eq in Heq_anonymous.
+                 subst.                 
+                 apply disjoint_symm in Daq.
+                 apply disjoint_symm in Dbq.
+                 rewrite <- manual_merge_assoc; trivial.
+                 apply disjoint_merge; trivial.
+                 apply pairwise_disjoint; assumption. Defined.
+Next Obligation. apply merge_eq. apply (merge_symm Mab). Defined.
 
 (* *)
